FiatFormal/Language/PreservationP.v
@@ -23,16 +23,46 @@ Proof.
   invert HS; intros.
   invert HT; intros; subst.
   invert H; intros; subst.
-  eapply subst_ADT_prog; invert H7; intros; subst.
-  simpl in *. eassumption.
-  eassumption.
-  assumption.
+
+  (* new *)
+  inversion H7; subst.
+  eapply subst_ADT_prog'; eauto.
+  cut (forall m t, TYPEMETHOD r ds nil nil m (substTT 0 r t)
+              -> TYPE ds nil nil (body m) (substTT 0 r t)); intros.
+  apply Forall2_map_left.
+  apply Forall2_map_right.
+  eapply Forall2_impl with (R1 := (fun m y => TYPEMETHOD r ds nil nil m (substTT 0 r y))).
+  intros. apply H. auto.
+  apply Forall2_map_right'.
+  apply mapCtor in H5; subst; auto.
+  intros. inversion H0; auto.
+  inversion H; subst. simpl; auto.
+  (* end new *)
+
   Case "PExp".
   invert HS; intros; subst.
   invert HT; intros; subst.
   apply TYExp.
   apply (preservation _ _ _ _ _ _ H4 H0).
 Qed.
+(* Proof. *)
+(*   intros pb ds pbOK p p' t HT HS. *)
+(*   gen pb ds pbOK p' t. *)
+(*   induction p; intros. *)
+(*   Case "PLet". *)
+(*   invert HS; intros. *)
+(*   invert HT; intros; subst. *)
+(*   invert H; intros; subst. *)
+(*   eapply subst_ADT_prog; invert H7; intros; subst. *)
+(*   simpl in *. eassumption. *)
+(*   eassumption. *)
+(*   assumption. *)
+(*   Case "PExp". *)
+(*   invert HS; intros; subst. *)
+(*   invert HT; intros; subst. *)
+(*   apply TYExp. *)
+(*   apply (preservation _ _ _ _ _ _ H4 H0). *)
+(* Qed. *)
 
 
 (* (* When we multi-step evaluate some expression, *)
