FiatFormal/Language/SubstExistential.v
@@ -4,6 +4,19 @@ Require Import FiatFormal.Language.SubstTypeExp.
 Require Import FiatFormal.Language.TyJudge.
 Require Import FiatFormal.Language.SubstTypeType.
 
+Lemma mapCtor {A : Type} :
+  forall (C : A -> A) xs xs',
+    (forall x x', C x = C x' -> x = x')
+    -> map C xs = map C xs'
+    -> xs = xs'.
+Proof.
+  induction xs;
+    destruct xs'; auto; try nope;
+      intros.
+  inversion H0.
+  f_equal. spec H H2; auto.
+  apply IHxs; auto.
+Qed.
 
 Theorem subst_exp_prog_ix :
   forall ds ke te t1 ix p t2 s,
@@ -19,23 +32,68 @@ Proof.
   apply TYLet.
   (* prove A generalized *)
   apply TYADT; try assumption.
+  apply (Forall2_map_left (TYPEMETHOD tr ds ke (delete ix te))).
+  apply (Forall2_map_right (fun (x : method) (y : ty) =>
+                              TYPEMETHOD tr ds ke (delete ix te) (substXM ix s x) y)).
+  apply (Forall2_impl_in (fun m t => TYPEMETHOD tr ds ke te m (substTT 0 tr t))); eauto; intros.
+  destruct x; simpl. inverts H4; subst. eapply TYMETHOD; eauto.
   eapply subst_value_value_ix; first [ eassumption; assumption ].
+  apply Forall2_map_right'; auto.
   (* prove B generalized *)
   unfold liftTE in *.
   rewrite map_delete.
-  rewrite delete_rewind.
+  rewrite delete_app.
+  apply mapCtor in H9; subst.
+  assert (length ms = length (map (substTT 0 tr) ts)).
+  eapply Forall2_length; eauto.
+  rewrite map_length in H. rewrite H.
   eapply IHTYPEPROG; simpl.
+  apply get_app_left_some.
   apply get_map.
   eassumption.
-  apply type_tyenv_weaken.
+  rewrite <- delete_app.
+  apply type_tyenv_weaken_append.
   rewrite <- map_delete.
   pose proof type_kienv_weaken.
-  unfold liftTE in H.
-  apply H. assumption.
+  unfold liftTE in H3.
+  apply H3. assumption.
+  (* injective cTor *)
+  intros; inversion H; auto.
   Case "PExp".
   apply TYExp.
   eapply subst_value_value_ix; first [ eassumption |  assumption].
 Qed.
+(* Theorem subst_exp_prog_ix : *)
+(*   forall ds ke te t1 ix p t2 s, *)
+(*     get ix te = Some t1 *)
+(*     -> TYPE ds ke (delete ix te) s t1 *)
+(*     -> TYPEPROG ds ke te p t2 *)
+(*     -> TYPEPROG ds ke (delete ix te) (substXP ix s p) t2. *)
+(* Proof. *)
+(*   intros. gen s ix t1. *)
+(*   induction H1; intros. *)
+(*   Case "PLet". *)
+(*   invert H; intros; subst; simpl. *)
+(*   apply TYLet. *)
+(*   (* prove A generalized *) *)
+(*   apply TYADT; try assumption. *)
+(*   eapply subst_value_value_ix; first [ eassumption; assumption ]. *)
+(*   (* prove B generalized *) *)
+(*   unfold liftTE in *. *)
+(*   rewrite map_delete. *)
+(*   rewrite delete_rewind. *)
+(*   eapply IHTYPEPROG; simpl. *)
+(*   apply get_map. *)
+(*   eassumption. *)
+(*   apply type_tyenv_weaken. *)
+(*   rewrite <- map_delete. *)
+(*   pose proof type_kienv_weaken. *)
+(*   unfold liftTE in H. *)
+(*   apply H. assumption. *)
+(*   Case "PExp". *)
+(*   apply TYExp. *)
+(*   eapply subst_value_value_ix; first [ eassumption |  assumption]. *)
+(* Qed. *)
 
 Theorem subst_exp_prog
   : forall ds ke te t1 p t2 s,
@@ -49,6 +107,66 @@ Proof.
   eapply subst_exp_prog_ix; simpl; eauto.
 Qed.
 
+(* new *)
+(* Substitution of several expressions at once. *)
+Theorem subst_exp_prog_list
+  : forall ds ks te ts p1 t1 xs,
+    Forall2 (TYPE ds ks te) xs ts
+    -> TYPEPROG ds ks (te >< ts) p1 t1
+    -> TYPEPROG ds ks te (substXXsP 0 xs p1) t1.
+Proof.
+  intros ds ks te ts p1 t1 xs HF HT.
+  gen ts ks p1.
+  induction xs; intros; invert_exp_type.
+
+  - Case "base case".
+    destruct ts.
+    + simpl. auto.
+    + nope.
+
+  - Case "step case".
+    simpl.
+    destruct ts.
+    + nope.
+    + inverts HF.
+      eapply IHxs.
+      * eauto.
+      * simpl in HT.
+        eapply subst_exp_prog.
+        eauto.
+        rrwrite (length xs = length ts).
+        eapply type_tyenv_weaken_append. auto.
+Qed.
+(* Theorem subst_exp_exp_list *)
+(*   : forall ds ks te x1 xs t1 ts, *)
+(*     Forall2 (TYPE ds ks te) xs ts *)
+(*     -> TYPE ds ks (te >< ts) x1 t1 *)
+(*     -> TYPE ds ks te (substXXs 0 xs x1) t1. *)
+(* Proof. *)
+(*   intros ds ks te x1 xs t1 ts HF HT. *)
+(*   gen ts ks x1. *)
+(*   induction xs; intros; invert_exp_type. *)
+
+(*   - Case "base case". *)
+(*     destruct ts. *)
+(*     + simpl. auto. *)
+(*     + nope. *)
+
+(*   - Case "step case". *)
+(*     simpl. *)
+(*     destruct ts. *)
+(*     + nope. *)
+(*     + inverts HF. *)
+(*       eapply IHxs. *)
+(*       * eauto. *)
+(*       * simpl in HT. *)
+(*         eapply subst_value_value. *)
+(*         eauto. *)
+(*         rrwrite (length xs = length ts). *)
+(*         eapply type_tyenv_weaken_append. auto. *)
+(* Qed. *)
+(* end new *)
+
 Theorem subst_type_prog_ix
   : forall ds ix ke kx S te p t,
     get ix ke = Some kx
@@ -61,38 +179,81 @@ Proof.
   Case "PLet".
   simpl. invert H; intros; subst.
   assert
-    (Hcomp : substTT (0 + ix) S (substTT 0 tr t2)
+    (Hcomp : forall ix S tr t, substTT (0 + ix) S (substTT 0 tr t)
              = (substTT 0 (substTT (0 + ix) S tr)
-                        (substTT (1 + 0 + ix) (liftTT 0 S) t2))).
-  apply substTT_substTT with (n:=0) (m:=ix).
+                        (substTT (1 + 0 + ix) (liftTT 0 S) t))); intros.
+  apply substTT_substTT with (n:=0) (m:=ix0).
   simpl in Hcomp.
   rewrite Hcomp.
+  (* new *)
+  rewrite map_map.
+  simpl. rewrite <- map_map with (f:=(substTT (Datatypes.S ix) (liftTT 0 S))).
+  (* end new *)
   apply TYLet.
   SCase "ADT".
+  (* new *)
+  (* rename t2 into t. *)
+  (* end new *)
   apply TYADT.
   eapply subst_type_type_ix.
   eassumption.
   assumption.
   assumption.
-  assert (Hcomp' : substTT (0 + ix) S (substTT 0 tr t)
-                   = (substTT 0 (substTT (0 + ix) S tr)
-                              (substTT (1 + 0 + ix) (liftTT 0 S) t))).
-  apply substTT_substTT with (n:=0) (m:=ix).
-  simpl in Hcomp'.
-  rewrite <- Hcomp'.
+
+  (* new *)
+  apply (Forall2_map_left (TYPEMETHOD (substTT ix S tr) ds (delete ix ke) (substTE ix S te))).
+  apply (Forall2_map_right (fun (x : method) (y : ty) =>
+                              TYPEMETHOD (substTT ix S tr) ds (delete ix ke) (substTE ix S te) (substTM ix S x) y)).
+  apply (Forall2_map_right (fun (x : method) (y : ty) =>
+     TYPEMETHOD (substTT ix S tr) ds (delete ix ke) (substTE ix S te) (substTM ix S x)
+       (substTT 0 (substTT ix S tr) y))).
+  apply (Forall2_impl_in (fun m t => TYPEMETHOD tr ds ke te m (substTT 0 tr t))); eauto; intros.
+  destruct x; simpl. inverts H4; subst.
+  rewrite <- Hcomp.
+  rewrite <- H16. simpl. (* needed to generalize Hcomp' for all ty -> In ty ts0 *)
+  rewrite map_app.
+  rewrite dup_map.
+
+  eapply TYMETHOD; eauto.
+  assert (Hsubst: (TNFun (dup (substTT ix S tr) arity >< map (substTT ix S) dom)
+                 (TNProd (nil :> substTT ix S tr :> substTT ix S tRes)))
+          = (substTT ix S (TNFun ((dup tr arity) >< dom) (TNProd (nil :> tr :> tRes)))));
+    simpl.
+  rewrite <- dup_map.
+  rewrite <- map_app.
+  auto.
+  rewrite Hsubst.
+  (* end new *)
+
   eapply subst_type_exp_ix.
   eassumption.
   assumption.
   assumption.
+
+  (* new *)
+  apply Forall2_map_right'; auto.
+  (* end new *)
+
   SCase "PROG".
   rewrite delete_rewind in *.
   rewrite liftTE_substTE with (n:=0) (n':=ix).
+
+  (* new *)
+  unfold substTE in *. rewrite <- map_app.
+  apply mapCtor in H9; subst.
+  (* end new *)
+
   eapply IHTYPEPROG.
   simpl.
   eassumption.
   simpl.
   eapply liftTT_weaken.
   assumption.
+
+  (* new *)
+  intros. inversion H; auto.
+  (* end new *)
+
   Case "PExp".
   apply TYExp.
   eapply subst_type_exp_ix.
@@ -100,6 +261,51 @@ Proof.
   assumption.
   assumption.
 Qed.
+(* Proof. *)
+  (* intros. gen S ix kx. *)
+  (* induction H1; intros. *)
+  (* Case "PLet". *)
+  (* simpl. invert H; intros; subst. *)
+  (* assert *)
+  (*   (Hcomp : substTT (0 + ix) S (substTT 0 tr t2) *)
+  (*            = (substTT 0 (substTT (0 + ix) S tr) *)
+  (*                       (substTT (1 + 0 + ix) (liftTT 0 S) t2))). *)
+  (* apply substTT_substTT with (n:=0) (m:=ix). *)
+  (* simpl in Hcomp. *)
+  (* rewrite Hcomp. *)
+  (* apply TYLet. *)
+  (* SCase "ADT". *)
+  (* apply TYADT. *)
+  (* eapply subst_type_type_ix. *)
+  (* eassumption. *)
+  (* assumption. *)
+  (* assumption. *)
+  (* assert (Hcomp' : substTT (0 + ix) S (substTT 0 tr t) *)
+  (*                  = (substTT 0 (substTT (0 + ix) S tr) *)
+  (*                             (substTT (1 + 0 + ix) (liftTT 0 S) t))). *)
+  (* apply substTT_substTT with (n:=0) (m:=ix). *)
+  (* simpl in Hcomp'. *)
+  (* rewrite <- Hcomp'. *)
+  (* eapply subst_type_exp_ix. *)
+  (* eassumption. *)
+  (* assumption. *)
+  (* assumption. *)
+  (* SCase "PROG". *)
+  (* rewrite delete_rewind in *. *)
+  (* rewrite liftTE_substTE with (n:=0) (n':=ix). *)
+  (* eapply IHTYPEPROG. *)
+  (* simpl. *)
+  (* eassumption. *)
+  (* simpl. *)
+  (* eapply liftTT_weaken. *)
+  (* assumption. *)
+  (* Case "PExp". *)
+  (* apply TYExp. *)
+  (* eapply subst_type_exp_ix. *)
+  (* eassumption. *)
+  (* assumption. *)
+  (* assumption. *)
+(* Qed. *)
 
 Theorem subst_type_prog
   : forall ds ke te X S p t,
@@ -133,5 +339,29 @@ Proof.
   specialize (STP HK).
   specialize (ESL x STP).
   specialize (ESL HT).
+  assumption.
+Qed.
+
+(* new *)
+Theorem subst_ADT_prog' :
+  forall ds X r kr ts t2 xs p,
+    TYPEPROG ds (nil :> X) (nil >< ts) p t2
+    -> KIND nil r kr
+    -> Forall2 (TYPE ds nil nil) xs (map (substTT 0 r) ts)
+    -> TYPEPROG ds nil nil (substXXsP 0 xs (substTP 0 r p)) (substTT 0 r t2).
+Proof.
+  intros ds X r kr ts t2 xs p HP HK HT.
+  pose proof (subst_type_prog) as STP.
+  specialize (STP _ _ _ _ r _ _ HP).
+  pose proof
+       (subst_exp_prog_list ds nil nil (map (substTT 0 r) ts) (substTP 0 r p) (substTT 0 r t2))
+    as ESL.
+  simpl in *.
+  destruct kr.
+  specialize (STP HK);
+    unfold substTE in STP.
+  rewrite map_app in STP; simpl in *.
+  specialize (ESL xs HT).
+  specialize (ESL STP).
   assumption.
 Qed.
